Updated a lot of stuff with a new definition for evaluation contexts

hoas.v
@@ -16,8 +16,7 @@ Reserved Notation "a '∉b' b" (at level 1, no associativity).
 Inductive NotInFV : string -> 𝔼 -> Prop :=
 | NotFVVarExpr {s1 s2} (neq : s1 <> s2) : s1 ∉f s2
 | NotFVNatExpr {s} {n : nat} : s ∉f n
-| NotFVAddExpr {s e1 e2} (notInLeft : s ∉f e1) (notInRight : s ∉f e2) : s ∉f (e1 + e2)
-| NotFVAppExpr {s e1 e2} (notInLeft : s ∉f e1) (notInRight : s ∉f e2) : s ∉f (AppExpr e1 e2)
+| NotFVBinExpr {s f e1 e2} (notInLeft : s ∉f e1) (notInRight : s ∉f e2) : s ∉f (BinExpr f e1 e2)
 | NotFVAbsExpru f x τarg τret body {s} (notF : f <> s) (notX : x <> s) (notInBody : s ∉f body) :
     s ∉f (AbsExpr f x τarg τret body)
 | NotFVAbsExprx f x τarg τret body : x ∉f (AbsExpr f x τarg τret body)
@@ -26,12 +25,10 @@ where "s ∉f e" := (NotInFV s e) : FV_scope.
 
 Inductive InFV : string -> 𝔼 -> Prop :=
 | FVVarExpr {s} : s ∈f s
-| FVAddExprL {s e1 e2} (inSub: s ∈f e1) : s ∈f (e1 + e2)
-| FVAddExprR {s e1 e2} (inSub: s ∈f e2) : s ∈f (e1 + e2)
+| FVBinExprL {s f e1 e2} (inSub: s ∈f e1) : s ∈f (BinExpr f e1 e2)
+| FVAddExprR {s f e1 e2} (inSub: s ∈f e2) : s ∈f (BinExpr f e1 e2)
 | FVAbsExpr {f x τarg τret body s} (notF : f <> s) (notX : x <> s) (inSub : s ∈f body) :
     s ∈f (AbsExpr f x τarg τret body)
-| FVAppExprL {s e1 e2} (inSub: s ∈f e1) : s ∈f (AppExpr e1 e2)
-| FVAppExprR {s e1 e2} (inSub: s ∈f e2) : s ∈f (AppExpr e1 e2)
 where "s ∈f e" := (InFV s e) : FV_scope.
 
 Open Scope FV_scope.
@@ -40,8 +37,7 @@ Fixpoint InFVb string expr :=
   match expr with
   | VarExpr s => if (string_dec string s) then true else false
   | NatExpr _ => false
-  | AddExpr e0 e1 => (InFVb string e0) || (InFVb string e1)
-  | AppExpr e0 e1 => (InFVb string e0) || (InFVb string e1)
+  | BinExpr f e0 e1 => (InFVb string e0) || (InFVb string e1)
   | AbsExpr f x _ _ body => if (string_dec string f) then
                              false
                            else if (string_dec string x) then
@@ -74,19 +70,15 @@ Inductive InBV : string -> 𝔼 -> Prop :=
 | BVFName {f x τarg τret body} : f ∈b (AbsExpr f x τarg τret body)
 | BVArg {f x τarg τret body} : x ∈b (AbsExpr f x τarg τret body)
 | BVBody {s f x τarg τret body} (inSub: s ∈b body) : s ∈b (AbsExpr f x τarg τret body)
-| BVAddExprL {s e1 e2} (inSub: s ∈b e1) : s ∈b (e1 + e2)
-| BVAddExprR {s e1 e2} (inSub: s ∈b e2) : s ∈b (e1 + e2)
-| BVAppExprL {s e1 e2} (inSub: s ∈b e1) : s ∈b (AppExpr e1 e2)
-| BVAppExprR {s e1 e2} (inSub: s ∈b e2) : s ∈b (AppExpr e1 e2)
+| BVBinExprL {s f e1 e2} (inSub: s ∈b e1) : s ∈b (BinExpr f e1 e2)
+| BVBinExprR {s f e1 e2} (inSub: s ∈b e2) : s ∈b (BinExpr f e1 e2)
 where "x ∈b e" := (InBV x e).
 
 Inductive NotInBV s : 𝔼 -> Prop :=
 | NotBVAbsExpr {f x τarg τret body} (notF : s <> f) (notX : s <> x) (notSub : s ∉b body)
   : s ∉b (AbsExpr f x τarg τret body)
-| NotBVAddExpr {e1 e2} (nsub1 : s ∉b e1) (nsub2: s ∉b e2)
-  : s ∉b (AddExpr e1 e2)
-| NotBVAppExpr {e1 e2} (nsub1 : s ∉b e1) (nsub2: s ∉b e2)
-  : s ∉b (AppExpr e1 e2)
+| NotBVBinExpr {f e1 e2} (nsub1 : s ∉b e1) (nsub2: s ∉b e2)
+  : s ∉b (BinExpr f e1 e2)
 | NotBVNatExpr (n : nat) : s ∉b n
 | NotBVVarExpr (s0 : string) : s ∉b s0
 where "s ∉b e" := (NotInBV s e).
@@ -95,8 +87,7 @@ Fixpoint InBVb s e :=
   match e with
   | VarExpr s => false
   | NatExpr n => false
-  | AddExpr l r => (InBVb s l)||(InBVb s r)
-  | AppExpr l r => (InBVb s l)||(InBVb s r)
+  | BinExpr f l r => (InBVb s l)||(InBVb s r)
   | AbsExpr f x τarg τret body =>
     if (string_dec s f) then true
     else if (string_dec s x) then true
@@ -124,14 +115,10 @@ Inductive CAS : 𝔼 -> string -> 𝔼 -> 𝔼 -> Prop :=
 | VarCASeq {s1 s2 e} (eq : s1 = s2) : [e / s1] s2 = e
 | VarCASneq {s1 s2 e} (neq : s1 <> s2) : [e / s1] s2 = s2
 | NatCAS {e s} (n : nat) : [e / s] n = n
-| AddCAS {e s e1 e1' e2 e2'}
-          (LeftAddCAS : [e / s] e1 = e1')
-          (RightAddCAS : [e / s] e2 = e2')
-  : [e / s] (e1 + e2) = (e1' + e2')
-| AppCAS {e s e1 e1' e2 e2'}
+| BinCAS {f e s e1 e1' e2 e2'}
           (LeftAppCAS : [e / s] e1 = e1')
           (RightAppCAS : [e / s] e2 = e2')
-  : [e / s] (AppExpr e1 e2) = (AppExpr e1' e2')
+  : [e / s] (BinExpr f e1 e2) = (BinExpr f e1' e2')
 | AbsCASUnbound {e s f x τarg τret body body'}
                 (notF : s <> f)
                 (notX : s <> x)
@@ -146,14 +133,11 @@ where "[ a / s ] b = c" := (CAS a s b c).
 Inductive SafeToSubInto (e : 𝔼) : 𝔼 -> Prop :=
 | SafeToSubIntoVarExpr {s : string} : SafeToSubInto e s
 | SafeToSubIntoNatExpr {n : nat} : SafeToSubInto e n
-| SafeToSubIntoAddExpr (e0 e1 : 𝔼)
+| SafeToSubIntoBinExpr (f : BinOp)
+                       (e0 e1 : 𝔼)
                        (safe1 : SafeToSubInto e e0)
                        (safe2 : SafeToSubInto e e1)
-  : SafeToSubInto e (e0 + e1)
-| SafeToSubIntoAppExpr (e0 e1 : 𝔼)
-                       (safe1 : SafeToSubInto e e0)
-                       (safe2 : SafeToSubInto e e1)
-  : SafeToSubInto e (AppExpr e0 e1)
+  : SafeToSubInto e (BinExpr f e0 e1)
 | SafeToSubIntoAbExpr {f x τarg τret body}
                       (notFIn : f ∉f e)
                       (notXIn : x ∉f e)
@@ -168,8 +152,7 @@ Lemma CASAlways {e1 x e} : SafeToSubInto e1 e -> exists e2, [e1 / x] e = e2.
     + exists e1 => //.
     + exists x0 => //.
   - move=> n; exists n => //.
-  - move=> e0 e2 ? [x0 ?] ? [x1 ?]; exists (AddExpr x0 x1) => //.
-  - move=> e0 e2 ? [x0 ?] ? [x1 ?]; exists (AppExpr x0 x1) => //.
+  - move=> f e0 e2 ? [x0 ?] ? [x1 ?]; exists (BinExpr f x0 x1) => //.
   - move=> f x0 τarg τret body fni x0ni safe [x2 ?].
     case: (string_dec x f) => [-> | nef].
     + exists (AbsExpr f x0 τarg τret body) => //.
@@ -191,6 +174,7 @@ Proof.
     + decide equality.
     + apply string_dec.
     + apply string_dec.
+    + decide equality.
 Qed.
 
 Inductive MultiCAS : substitution_list -> 𝔼 -> 𝔼 -> Prop :=
@@ -204,14 +188,10 @@ Reserved Notation "a '≡α' b" (at level 1, no associativity).
 
 Inductive AlphaEquiv : 𝔼 -> 𝔼 -> Prop :=
 | RAE {e} : e ≡α e 
-| AAE {a b c d}
+| PAE {f a b c d}
       (AEQac : a ≡α c)
       (AEQbd : b ≡α d)
-  : (a + b) ≡α (c + d)
-| PAE {a b c d}
-      (AEQac : a ≡α c)
-      (AEQbd : b ≡α d)
-  : (AppExpr a b) ≡α (AppExpr c d)
+  : (BinExpr f a b) ≡α (BinExpr f c d)
 | BAE {f f1 f2 x x1 x2 τarg τret body1 body1' body2 body2'}
       (FXDiff : f <> x)
       (FFresh1 : f ∉f body1)
