lang.v
@@ -22,19 +22,20 @@ Bind Scope LType_scope with LType.
 Notation "'ℕ'" := NatType : LType_scope.
 Notation "a → b" := (AbsType a b) (at level 50, left associativity) : LType_scope.
 
+Inductive BinOp : Set := AddExpr | AppExpr.
+
 Inductive Expression : Set :=
 | VarExpr (x : string) : Expression
 | NatExpr (n : nat) : Expression
-| AddExpr (e1 e2 : Expression) : Expression
 | AbsExpr (f x : string) (τarg τret : LType) (body : Expression) : Expression
-| AppExpr (e1 e2 : Expression) : Expression.
+| BinExpr (f : BinOp) (e1 e2 : Expression) : Expression.
 
 Coercion VarExpr : string >-> Expression.
 Coercion NatExpr : nat >-> Expression.
 Bind Scope Expression_scope with Expression.
-Arguments AddExpr (e1 e2)%Expression_scope.
+Arguments BinExpr f (e1 e2)%Expression_scope.
 Arguments AbsExpr (f x)%string_scope (τarg τret)%LType_scope body%Expression_scope.
-Notation "a + b" := (AddExpr a b) : Expression_scope.
+Notation "a + b" := (BinExpr AddExpr a b) : Expression_scope.
 
 Inductive LValue : Expression -> Prop :=
 | NatValue n: LValue (NatExpr n)
@@ -42,21 +43,16 @@ Inductive LValue : Expression -> Prop :=
 
 Inductive EvaluationContext : Set :=
 | Hole : EvaluationContext
-| EvalContextLAdd (E : EvaluationContext) (e : Expression) : EvaluationContext
-| EvalContextRAdd (n : nat) (E : EvaluationContext) : EvaluationContext
-| EvalContextLApp (E : EvaluationContext) (e : Expression) : EvaluationContext
-| EvalContextRApp (f x : string) (τarg τret : LType) (body : Expression) (E : EvaluationContext) : EvaluationContext.
+| EvalContextBinL (f : BinOp) (E : EvaluationContext) (e : Expression) : EvaluationContext
+| EvalContextBinR (f : BinOp) {e} (v : LValue e) (E : EvaluationContext) : EvaluationContext.
 
 Reserved Notation "E [ e ]" (at level 0, e at next level).
 
 Fixpoint FillEvaluationContext E e :=
   match E with
   | Hole => e
-  | EvalContextLAdd E0 e0 => (AddExpr E0[e] e0)
-  | EvalContextRAdd n E0 => (AddExpr n E0[e])
-  | EvalContextLApp E0 e0 => (AppExpr E0[e] e0)
-  | EvalContextRApp f x τarg τbody body E0 =>
-    (AppExpr (AbsExpr f x τarg τbody body) E0[e])
+  | EvalContextBinL f E0 e0 => BinExpr f (E0 [e]) e0
+  | @EvalContextBinR f e0 v E0 => BinExpr f e0 (E0 [e])
   end
 where "E [ e ]" := (FillEvaluationContext E e).
 
